Refactor ReducibilityRenaming proof

ReducibilityRenaming.v
@@ -42,187 +42,376 @@ Opaque reducible_values.
 Opaque makeFresh.
 Opaque lt.
 
-Ltac t_apply_ih :=
-  lazymatch goal with
-  | IH: forall m, _ -> forall T T' t theta theta' l, _ ,
-    H1: reducible_values ?theta' ?t ?T',
-    H2: equal_with_relation ?rel ?T ?T' |-
-      reducible_values ?theta ?t ?T =>
-        unshelve eapply (IH (size T, index T) _ T T' t theta theta' rel); eauto
-  | IH: forall m, _ -> forall T T' t theta theta' l, _ ,
-    H1: reducible_values ?theta ?t ?T,
-    H2: equal_with_relation ?rel ?T ?T' |-
-      reducible_values ?theta' ?t ?T' =>
-        unshelve eapply (IH (size T, index T) _ T T' t theta theta' rel); eauto
-  end.
-
-Ltac t_apply_ih2 :=
-  lazymatch goal with
-  | IH: forall m, _ -> forall T T' t theta theta' l, _ ,
-    H1: reducible_values ?theta' ?t ?T',
-    H2: equivalent_with_relation ?rel ?theta ?theta' _ |-
-      reducible_values ?theta ?t ?T =>
-        unshelve eapply (IH (size T, index T) _ T T' t theta theta' rel); eauto
-  | IH: forall m, _ -> forall T T' t theta theta' l, _ ,
-    H1: reducible_values ?theta ?t ?T,
-    H2: equivalent_with_relation ?rel ?theta ?theta' _ |-
-      reducible_values ?theta' ?t ?T' =>
-        unshelve eapply (IH (size T, index T) _ T T' t theta theta' rel); eauto
-  end.
-
-Set Program Mode.
-
 Ltac t_bewr_constructor :=
   match goal with
   | |- equal_with_relation _ _ _ => constructor
   end.
 
-Lemma reducible_rename_aux:
-  forall measure T T' t (theta theta' : interpretation) rel,
-    (size T, index T) = measure ->
+(* The property that we wnat to prove for a type T and a measure m *)
+Definition renamable_prop m T: Prop :=
+  forall (T' t : tree) (theta theta' : interpretation) (rel : map nat nat),
+    (size T, index T) = m ->
     valid_interpretation theta ->
     valid_interpretation theta' ->
     equivalent_with_relation rel theta theta' equivalent_rc ->
     equal_with_relation rel T T' ->
-    (
-      reducible_values theta t T <->
-      reducible_values theta' t T'
-    ).
+      (reducible_values theta t T <-> reducible_values theta' t T').
+
+Definition renamable_prop_IH m: Prop := forall m', m' << m -> forall T', renamable_prop m' T'.
+
+Lemma reducible_rename_induct:
+  forall (theta theta' : interpretation) (rel : map nat nat) A A' v n1 n2,
+    renamable_prop_IH (n1, n2) ->
+    equal_with_relation rel A A' ->
+    equivalent_with_relation rel theta theta' equivalent_rc ->
+    reducible_values theta v A ->
+    valid_interpretation theta ->
+    valid_interpretation theta' ->
+    size A < n1 ->
+    reducible_values theta' v A'.
 Proof.
-  induction measure using measure_induction; intros; destruct T;
-      repeat match goal with
-      | _ => step || t_fv_open ||  simp_red || t_listutils || t_lookup || destruct_tag
-      | _ => apply equal_with_relation_open
-      | _ => apply left_lex
-      | _ => t_instantiate_rel
-      | _ => t_lookup_same
-      | _ => t_equal_with_erased
-      | _ => step_inversion equal_with_relation
-      | _ => t_apply_ih
-      | _ => find_exists || find_smallstep_value
-      | H: is_erased_term ?t |- _ => rewrite (is_erased_subst t) in *
-      | _ => apply erased_is_erased
-      | _ => rewrite erased_term_tfv in *
-      | _ => progress ( autorewrite with bsize in * )
-      | _ => rewrite substitute_open2 in * by
-            (repeat step || ( rewrite erased_term_tfv in * ) ||
-                    eauto using is_renaming_twfs, is_renaming_wfs)
-      | IH: forall m, _ -> forall T T' t theta theta' l, _ ,
-        H1: reducible_values ?theta' ?t (open 0 ?T' ?a) ,
-        H2: equal_with_relation ?rel ?T ?T' |-
-          reducible_values ?theta ?t (open 0 ?T ?a) =>
-            unshelve eapply (IH _ _ (open 0 T a) (open 0 T' a) t theta theta' rel); eauto
-      | IH: forall m, _ -> forall T T' t theta theta' l, _ ,
-        H1: reducible_values ?theta ?t (open 0 ?T ?a),
-        H2: equal_with_relation ?rel ?T ?T' |-
-          reducible_values ?theta' ?t (open 0 ?T' ?a) =>
-            unshelve eapply (IH _ _ (open 0 T a) (open 0 T' a) t theta theta' rel); eauto
-      | _: is_erased_term ?b, H: forall a, _ -> _ -> reduces_to (fun t => reducible_values ?theta t (open 0 ?T _)) _ |-
-          reduces_to _ _ =>
-        poseNew (Mark 0 "reduces_to_equiv");
-        apply reduces_to_equiv with (fun t => reducible_values theta t (open 0 T b))
-      | |- _ ∈ support _ => apply_any
-      | H: forall a, _ -> reduces_to _ _ |- _ => apply H
-      | H: forall a, _ -> reducible_values _ _ _ |- _ => apply H
-      | H1: forall a, is_erased_term a -> reducible_values _ _ _ -> _,
-        H2: is_erased_term ?a  |- _ =>
-          poseNew (Mark H1 "instantiate");
-          unshelve epose proof (H1 a _ _)
-      | |- exists c d _, pp ?a ?b = pp _ _ /\ _ => unshelve exists a, b
-      | H: star small_step _ ?a |- _ => is_var a; unshelve exists a (* !! *)
-(*      | H: is_erased_term ?a |- _ => unshelve exists a (* !! *) *)
-      | H1: equal_with_relation _ ?T ?T',
-        H: reducible_values _ ?t ?T |- exists _ _, reducible_values _ _ ?T' /\ _ => exists t
-      | H1: equal_with_relation _ ?T' ?T,
-        H: reducible_values _ ?t ?T |- exists _ _, reducible_values _ _ ?T' /\ _ => exists t
-      | H1: equal_with_relation _ ?T ?T',
-        H: reducible_values _ ?t ?T |- reducible_values _ ?t ?T' \/ _ => left
-      | H1: equal_with_relation _ ?T' ?T,
-        H: reducible_values _ ?t ?T |- reducible_values _ ?t ?T' \/ _ => left
-      | H1: equal_with_relation _ ?T ?T',
-        H: reducible_values _ ?t ?T |- _ \/ reducible_values _ ?t ?T' => right
-      | H1: equal_with_relation _ ?T' ?T,
-        H: reducible_values _ ?t ?T |- _ \/ reducible_values _ ?t ?T' => right
-      | H1: equal_with_relation _ ?T ?T',
-        H: reducible_values _ ?t (open _ ?T _) |- exists _, reducible_values _ _ (open _ ?T' _) => exists t
-      | H1: equal_with_relation _ ?T' ?T,
-        H: reducible_values _ ?t (open _ ?T _) |- exists _, reducible_values _ _ (open _ ?T' _) => exists t
-      | H: star small_step _ zero |- _ \/ _ => left
-      | H: star small_step _ (succ _) |- _ => right
-      | H1: equal_with_relation ?rel ?T ?T' |- exists X, (X ∈ ?L -> False) /\ _ =>
-          exists (makeFresh (L :: (range rel) :: (range (swap rel)) :: (pfv T type_var) :: (pfv T' type_var) :: nil))
-      | |- (exists v, tleft ?v' = tleft v /\ _) \/ _ => left; exists v'
-      | |- _ \/ (exists v, tright ?v' = tright v /\ _) => right; exists v'
-      end;
+  unfold renamable_prop_IH; intros.
+  match goal with
+  | IH: forall m, _ << _ -> _ ,
+    H1: reducible_values ?theta ?t ?T,
+    H2: equal_with_relation ?rel ?T ?T' |-
+      reducible_values ?theta' ?t ?T' =>
+        unshelve eapply (IH (size T, index T) _ T T' t theta theta' rel); eauto
+  end.
+  repeat step || apply left_lex.
+Qed.
+
+Lemma reducible_rename_induct_back:
+  forall (theta theta' : interpretation) (rel : map nat nat) A A' v n1 n2,
+    renamable_prop_IH (n1, n2) ->
+    equal_with_relation rel A A' ->
+    equivalent_with_relation rel theta theta' equivalent_rc ->
+    reducible_values theta' v A' ->
+    valid_interpretation theta ->
+    valid_interpretation theta' ->
+    size A < n1 ->
+    reducible_values theta v A.
+Proof.
+  unfold renamable_prop_IH; intros.
+  match goal with
+  | IH: forall m, _ << _ -> _ ,
+    H1: reducible_values ?theta' ?t ?T',
+    H2: equal_with_relation ?rel ?T ?T' |-
+      reducible_values ?theta ?t ?T =>
+        unshelve eapply (IH (size T, index T) _ T T' t theta theta' rel); eauto
+  end.
+  repeat step || apply left_lex.
+Qed.
+
+Ltac t_apply_ih :=
+  lazymatch goal with
+  | IH: forall m, _ << _ -> _ ,
+    H1: reducible_values ?theta' ?t ?T',
+    H2: equivalent_with_relation ?rel ?theta ?theta' _ |-
+      reducible_values ?theta ?t ?T =>
+        unshelve eapply (IH (size T, index T) _ T T' t theta theta' rel); eauto
+  | IH: forall m, _ << _ -> _ ,
+    H1: reducible_values ?theta ?t ?T,
+    H2: equivalent_with_relation ?rel ?theta ?theta' _ |-
+      reducible_values ?theta' ?t ?T' =>
+        unshelve eapply (IH (size T, index T) _ T T' t theta theta' rel); eauto
+  end.
+
+Lemma reducible_rename_induct_open:
+  forall (theta theta' : interpretation) (rel : map nat nat) B B' v a n1 n2,
+    renamable_prop_IH (n1, n2) ->
+    equal_with_relation rel B B' ->
+    equivalent_with_relation rel theta theta' equivalent_rc ->
+    reducible_values theta v (open 0 B a) ->
+    valid_interpretation theta ->
+    valid_interpretation theta' ->
+    is_erased_term a ->
+    size (open 0 B a) < n1 ->
+    reducible_values theta' v (open 0 B' a).
+Proof.
+  unfold renamable_prop_IH; intros.
+  t_apply_ih; repeat step || apply left_lex || apply equal_with_relation_open; eauto with bfv.
+Qed.
+
+Lemma reducible_rename_induct_open_back:
+  forall (theta theta' : interpretation) (rel : map nat nat) B B' v a n1 n2,
+    renamable_prop_IH (n1, n2) ->
+    equal_with_relation rel B B' ->
+    equivalent_with_relation rel theta theta' equivalent_rc ->
+    reducible_values theta' v (open 0 B' a) ->
+    valid_interpretation theta ->
+    valid_interpretation theta' ->
+    is_erased_term a ->
+    size (open 0 B a) < n1 ->
+    reducible_values theta v (open 0 B a).
+Proof.
+  unfold renamable_prop_IH; intros.
+  t_apply_ih; repeat step || apply left_lex || apply equal_with_relation_open; eauto with bfv.
+Qed.
+
+Ltac t_induct :=
+  solve [ eapply reducible_rename_induct; eauto 1; steps; try omega ].
+
+Ltac t_induct_back :=
+  solve [ eapply reducible_rename_induct_back; eauto 1; steps; try omega ].
+
+Ltac t_induct_open :=
+  solve [ eapply reducible_rename_induct_open; eauto 1; repeat step || autorewrite with bsize; try omega; eauto 2 with berased ].
+
+Ltac t_induct_open_back :=
+  solve [ eapply reducible_rename_induct_open_back; eauto 1; repeat step || autorewrite with bsize; try omega; eauto 2 with berased ].
+
+Ltac t_induct_all := t_induct || t_induct_back || t_induct_open || t_induct_open_back.
+
+Ltac t_prove_reduces_to :=
+  match goal with
+  | H: forall a, _ -> _ -> reduces_to _ _ |- _ => apply H; eauto 2 with berased; [ idtac ]
+  | H: forall a, _ -> _ -> reduces_to _ _ |- _ => apply H; eauto 2 with berased; fail
+  end.
+
+Lemma reducible_rename_reduces_to:
+  forall (T1 T2 t : tree) (theta theta' : interpretation) (rel : map nat nat) A' B' a,
+    equivalent_with_relation rel theta theta' equivalent_rc ->
+    renamable_prop_IH (S (S (S (size T1 + size T2))), None) ->
+    reducible_values theta' a A' ->
+    valid_interpretation theta ->
+    valid_interpretation theta' ->
+    (forall a : tree,
+        is_erased_term a ->
+        reducible_values theta a T1 ->
+        reduces_to (fun t0 : tree => reducible_values theta t0 (open 0 T2 a)) (app t a)) ->
+    equal_with_relation rel T1 A' ->
+    equal_with_relation rel T2 B' ->
+    reduces_to (fun t0 : tree => reducible_values theta' t0 (open 0 B' a)) (app t a).
+Proof.
+  intros.
+  repeat step || t_reduces_to || t_reduces_to2 || t_prove_reduces_to || t_induct_all.
+Qed.
+
+Lemma reducible_rename_reduces_to_back:
+  forall (T1 T2 t : tree) (theta theta' : interpretation) (rel : map nat nat) A' B' a,
+    equivalent_with_relation rel theta theta' equivalent_rc ->
+    renamable_prop_IH (S (S (S (size T1 + size T2))), None) ->
+    reducible_values theta a T1 ->
+    valid_interpretation theta ->
+    valid_interpretation theta' ->
+    (forall a : tree,
+        is_erased_term a ->
+        reducible_values theta' a A' ->
+        reduces_to (fun t0 : tree => reducible_values theta' t0 (open 0 B' a)) (app t a)) ->
+    equal_with_relation rel T1 A' ->
+    equal_with_relation rel T2 B' ->
+    reduces_to (fun t0 : tree => reducible_values theta t0 (open 0 T2 a)) (app t a).
+Proof.
+  intros.
+  repeat step || t_reduces_to || t_reduces_to2 || t_prove_reduces_to || t_induct_all.
+Qed.
+
+Lemma reducible_rename_fvar: forall m n f, renamable_prop_IH m -> renamable_prop m (fvar n f).
+Proof.
+  unfold renamable_prop;
+  repeat step || destruct_tag || step_inversion equal_with_relation || simp_red || t_lookup || t_lookup_same || t_instantiate_rel;
+    try solve [ eapply equivalent_rc_left; eauto 1 ];
+    try solve [ eapply equivalent_rc_right; eauto 1 ].
+Qed.
+
+Hint Immediate reducible_rename_fvar: b_rename.
+
+Lemma reducible_rename_arrow: forall m T1 T2, renamable_prop_IH m -> renamable_prop m (T_arrow T1 T2).
+Proof.
+  unfold renamable_prop;
+  repeat step || simp_red || step_inversion equal_with_relation;
+    eauto 2 using reducible_rename_reduces_to;
+    eauto 2 using reducible_rename_reduces_to_back.
+Qed.
+
+Hint Immediate reducible_rename_arrow: b_rename.
+
+Lemma reducible_rename_prod: forall m T1 T2, renamable_prop_IH m -> renamable_prop m (T_prod T1 T2).
+Proof.
+  unfold renamable_prop;
+  repeat step || simp_red || step_inversion equal_with_relation || find_exists || t_induct_all.
+Qed.
+
+Hint Immediate reducible_rename_prod: b_rename.
+
+Lemma reducible_rename_sum: forall m T1 T2, renamable_prop_IH m -> renamable_prop m (T_sum T1 T2).
+Proof.
+  unfold renamable_prop;
+  repeat step || simp_red || step_inversion equal_with_relation || find_exists || t_induct_all.
+Qed.
+
+Hint Immediate reducible_rename_sum: b_rename.
+
+Lemma reducible_rename_refine: forall m T b, renamable_prop_IH m -> renamable_prop m (T_refine T b).
+Proof.
+  unfold renamable_prop;
+  repeat step || simp_red || step_inversion equal_with_relation || t_induct_all || t_equal_with_erased.
+Qed.
+
+Hint Immediate reducible_rename_refine: b_rename.
+
+Lemma reducible_rename_type_refine: forall m T1 T2, renamable_prop_IH m -> renamable_prop m (T_type_refine T1 T2).
+Proof.
+  unfold renamable_prop;
+  repeat step || simp_red || step_inversion equal_with_relation || t_induct_all || find_exists_open.
+Qed.
+
+Hint Immediate reducible_rename_type_refine: b_rename.
+
+Lemma reducible_rename_let: forall m t T, renamable_prop_IH m -> renamable_prop m (T_let t T).
+Proof.
+  unfold renamable_prop;
+  repeat step || simp_red || step_inversion equal_with_relation || t_induct_all || find_smallstep_value2 || t_equal_with_erased.
+Qed.
+
+Hint Immediate reducible_rename_let: b_rename.
+
+Lemma reducible_rename_singleton: forall m t, renamable_prop_IH m -> renamable_prop m (T_singleton t).
+Proof.
+  unfold renamable_prop;
+  repeat step || simp_red || step_inversion equal_with_relation || t_induct_all || t_equal_with_erased.
+Qed.
+
+Hint Immediate reducible_rename_singleton: b_rename.
+
+Lemma reducible_rename_intersection: forall m T1 T2, renamable_prop_IH m -> renamable_prop m (T_intersection T1 T2).
+Proof.
+  unfold renamable_prop;
+  repeat step || simp_red || step_inversion equal_with_relation || t_induct_all.
+Qed.
+
+Hint Immediate reducible_rename_intersection: b_rename.
+
+Lemma reducible_rename_union: forall m T1 T2, renamable_prop_IH m -> renamable_prop m (T_union T1 T2).
+Proof.
+  unfold renamable_prop;
+  repeat match goal with
+         | H1: equal_with_relation _ ?T ?T',
+           H: reducible_values _ ?t ?T |- reducible_values _ ?t ?T' \/ _ => left
+         | H1: equal_with_relation _ ?T' ?T,
+           H: reducible_values _ ?t ?T |- reducible_values _ ?t ?T' \/ _ => left
+         | H1: equal_with_relation _ ?T ?T',
+           H: reducible_values _ ?t ?T |- _ \/ reducible_values _ ?t ?T' => right
+         | H1: equal_with_relation _ ?T' ?T,
+           H: reducible_values _ ?t ?T |- _ \/ reducible_values _ ?t ?T' => right
+         | _ => step || simp_red || step_inversion equal_with_relation || t_induct_all || find_exists
+         end.
+Qed.
+
+Hint Immediate reducible_rename_union: b_rename.
+
+Lemma reducible_rename_equal: forall m t1 t2, renamable_prop_IH m -> renamable_prop m (T_equal t1 t2).
+Proof.
+  unfold renamable_prop;
+  repeat step || simp_red || step_inversion equal_with_relation || t_induct_all || t_equal_with_erased.
+Qed.
+
+Hint Immediate reducible_rename_equal: b_rename.
+
+Lemma reducible_rename_forall: forall m T1 T2, renamable_prop_IH m -> renamable_prop m (T_forall T1 T2).
+Proof.
+  unfold renamable_prop;
+  repeat step || simp_red || step_inversion equal_with_relation || t_induct_all || t_instantiate_reducible_erased.
+Qed.
+
+Hint Immediate reducible_rename_forall: b_rename.
+
+Lemma reducible_rename_exists: forall m T1 T2, renamable_prop_IH m -> renamable_prop m (T_exists T1 T2).
+Proof.
+  unfold renamable_prop;
+  repeat match goal with
+         | H1: equal_with_relation _ ?T ?T',
+           H: reducible_values _ ?t ?T |- exists _ _, reducible_values _ _ ?T' /\ _ => exists t
+         | H1: equal_with_relation _ ?T' ?T,
+           H: reducible_values _ ?t ?T |- exists _ _, reducible_values _ _ ?T' /\ _ => exists t
+         | _ => step || simp_red || step_inversion equal_with_relation || t_induct_all
+         end.
+Qed.
+
+Hint Immediate reducible_rename_exists: b_rename.
+
+Lemma reducible_rename_type_abs: forall m T, renamable_prop_IH m -> renamable_prop m (T_abs T).
+Proof.
+  unfold renamable_prop, renamable_prop_IH;
+  repeat match goal with
+         | H1: equal_with_relation ?rel ?T ?T' |- exists X, (X ∈ ?L -> False) /\ _ =>
+             exists (makeFresh (L :: (range rel) :: (range (swap rel)) :: (pfv T type_var) :: (pfv T' type_var) :: nil))
+         | _ => step || simp_red || step_inversion equal_with_relation
+         end; try finisher.
+
+  - instantiate_any. eapply reduces_to_equiv; eauto 1; steps.
+    lazymatch goal with
+    | IH: forall m, _ << _ ->  _ ,
+      H1: reducible_values ((?X,?RC) :: ?theta) ?t ?T,
+      H2: equal_with_relation ?rel _ _ |-
+        reducible_values ((?M,?RC) :: ?theta') ?t ?T' =>
+          unshelve epose proof
+            (IH (size T, index T) _ T T' t
+                 ((X,RC) :: theta)
+                 ((M,RC) :: theta')
+                 ((X,M) :: rel)
+                 _ _ _ _ _
+            )
+    end;
+      repeat
+        steps || (progress autorewrite with bsize in * ) || t_fv_open || t_listutils ||
+        apply equivalent_with_relation_add || finisher ||
+        apply equal_with_relation_topen ||
+        apply left_lex ||
+        (rewrite substitute_topen3 in * by steps);
       try omega;
-      try finisher;
-      eauto with falsity;
-      eauto with bwf;
-      eauto with bfv;
-      try solve [ eapply equivalent_rc_left; eauto 1 ];
-      try solve [ eapply equivalent_rc_right; eauto 1 ];
-      t_closer.
+      eauto using in_remove_support;
+      eauto using equivalent_rc_refl.
 
-    - instantiate_any. eapply reduces_to_equiv; eauto 1; steps.
-      lazymatch goal with
-      | IH: forall m, _ -> forall T T' t theta theta' rel, _ ,
-        H1: reducible_values ((?X,?RC) :: ?theta) ?t ?T,
-        H2: equal_with_relation ?rel _ _ |-
-          reducible_values ((?M,?RC) :: ?theta') ?t ?T' =>
-            unshelve epose proof
-              (IH (size T, index T) _ T T' t
-                   ((X,RC) :: theta)
-                   ((M,RC) :: theta')
-                   ((X,M) :: rel)
-                   _ _ _ _ _
-              )
-      end;
-        repeat
-          steps || (progress autorewrite with bsize in * ) || t_fv_open || t_listutils ||
-          apply equivalent_with_relation_add || finisher ||
-          apply equal_with_relation_topen ||
-          apply left_lex ||
-          (rewrite substitute_topen3 in * by steps);
-        try omega;
-        eauto using in_remove_support;
-        eauto using equivalent_rc_refl.
+  - instantiate_any. eapply reduces_to_equiv; eauto 1; steps.
+    lazymatch goal with
+    | IH: forall m, _ << _ ->  _ ,
+      H1: reducible_values ((?X,?RC) :: ?theta) ?t ?T,
+      H2: equal_with_relation ?rel _ _ |-
+        reducible_values ((?M,?RC) :: ?theta') ?t ?T' =>
+          unshelve epose proof
+            (IH (size T, index T) _ T T' t
+                 ((X,RC) :: theta)
+                 ((M,RC) :: theta')
+                 ((X,M) :: (swap rel))
+                 _ _ _ _ _
+            )
+    end;
+      repeat
+        steps || (progress autorewrite with bsize in * ) || t_fv_open || t_listutils ||
+        apply equivalent_with_relation_add || finisher ||
+        apply equal_with_relation_topen ||
+        apply equivalent_with_relation_swap ||
+        apply equal_with_relation_swap ||
+        apply left_lex ||
+        match goal with
+        | H: equal_with_relation _ _ _ |- _ =>
+          rewrite (equal_with_relation_size _ _ _ H) in * by steps
+        end ||
+        (rewrite substitute_topen3 in * by steps);
+      try omega;
+      eauto using in_remove_support;
+      eauto using equivalent_rc_refl;
+      eauto 2 using equivalent_rc_sym.
+Qed.
 
-    - instantiate_any. eapply reduces_to_equiv; eauto 1; steps.
-      lazymatch goal with
-      | IH: forall m, _ -> forall T T' t theta theta' rel, _ ,
-        H1: reducible_values ((?X,?RC) :: ?theta) ?t ?T,
-        H2: equal_with_relation ?rel _ _ |-
-          reducible_values ((?M,?RC) :: ?theta') ?t ?T' =>
-            unshelve epose proof
-              (IH (size T, index T) _ T T' t
-                   ((X,RC) :: theta)
-                   ((M,RC) :: theta')
-                   ((X,M) :: (swap rel))
-                   _ _ _ _ _
-              )
-      end;
-        repeat
-          steps || (progress autorewrite with bsize in * ) || t_fv_open || t_listutils ||
-          apply equivalent_with_relation_add || finisher ||
-          apply equal_with_relation_topen ||
-          apply equivalent_with_relation_swap ||
-          apply equal_with_relation_swap ||
-          apply left_lex ||
-          match goal with
-          | H: equal_with_relation _ _ _ |- _ =>
-            rewrite (equal_with_relation_size _ _ _ H) in * by steps
-          end ||
-          (rewrite substitute_topen3 in * by steps);
-        try omega;
-        eauto using in_remove_support;
-        eauto using equivalent_rc_refl;
-        eauto 2 using equivalent_rc_sym.
+Hint Immediate reducible_rename_type_abs: b_rename.
+
+Lemma reducible_rename_rec: forall m n T0 Ts, renamable_prop_IH m -> renamable_prop m (T_rec n T0 Ts).
+Proof.
+  unfold renamable_prop, renamable_prop_IH;
+  repeat match goal with
+         | H: star small_step _ zero |- _ \/ _ => left
+         | H: star small_step _ (succ _) |- _ => right
+         | _ => step || simp_red || step_inversion equal_with_relation || t_equal_with_erased || find_exists || t_induct_all
+         end.
 
   - (* case recursive type at n + 1 *)
     unshelve eexists n', v', (makeFresh (pfv T0' type_var :: pfv Ts' type_var ::  support theta' :: nil)), _, _; eauto;
       repeat step || finisher.
     lazymatch goal with
-    | IH: forall m, _ -> forall T T' t theta theta' rel, _ ,
+    | IH: forall m, _ << _ -> _ ,
       H1: reducible_values ((?X,?RC1) :: ?theta) ?t ?T,
       H2: equal_with_relation ?rel _ _ |-
         reducible_values ((?M,?RC2) :: ?theta') ?t ?T' =>
@@ -241,7 +430,7 @@ Proof.
         unfold equivalent_rc ||
         apply equal_with_relation_refl ||
         (rewrite substitute_topen3 in * by steps) ||
-        t_apply_ih2 || t_bewr_constructor;
+        t_apply_ih || t_bewr_constructor;
       try solve [ apply left_lex; omega ];
       try solve [ apply right_lex; apply lt_index_step; auto ];
       eauto using in_remove_support;
@@ -249,10 +438,10 @@ Proof.
       eauto with bfv.
 
   - (* case recursive type at n + 1 *)
-   unshelve eexists n'0, v', (makeFresh (pfv T2 type_var :: pfv T3 type_var :: support theta :: nil)), _, _; eauto;
+   unshelve eexists n'0, v', (makeFresh (pfv T0 type_var :: pfv Ts type_var :: support theta :: nil)), _, _; eauto;
       repeat step || finisher.
     lazymatch goal with
-    | IH: forall m, _ -> forall T T' t theta theta' rel, _ ,
+    | IH: forall m, _ << _ ->  _ ,
       H1: reducible_values ((?X,?RC1) :: ?theta) ?t ?T,
       H2: equal_with_relation ?rel _ _ |-
         reducible_values ((?M,?RC2) :: ?theta') ?t ?T' =>
@@ -277,13 +466,22 @@ Proof.
           rewrite (equal_with_relation_size _ _ _ H) in * by steps
         end ||
         (rewrite substitute_topen3 in * by steps) ||
-        t_apply_ih2 || t_bewr_constructor;
+        t_apply_ih || t_bewr_constructor;
       try solve [ apply left_lex; omega ];
       try solve [ apply right_lex; apply lt_index_step; auto ];
       eauto using in_remove_support;
       eauto using reducibility_is_candidate;
       eauto with bfv;
       try solve [ apply_any; assumption ].
+Qed.
+
+Hint Immediate reducible_rename_rec: b_rename.
+
+Lemma reducible_rename_aux: forall m T, renamable_prop m T.
+Proof.
+  induction m using measure_induction; destruct T;
+    eauto 2 with b_rename;
+    try solve [ unfold renamable_prop; repeat step || simp_red || step_inversion equal_with_relation ].
 Qed.
 
 Lemma reducible_rename :
@@ -295,7 +493,7 @@ Lemma reducible_rename :
     equal_with_relation rel T T' ->
     reducible_values theta' t T'     .
 Proof.
-  intros; eapply (reducible_rename_aux _ T T' t theta theta' rel); eauto.
+  intros; eapply (reducible_rename_aux _ T T' t theta theta' rel); eauto 1.
 Qed.
 
 Lemma reducible_rename_one:
